Attempt to get CF div project unstuck

examples/divLoopScript.sml
@@ -7,21 +7,11 @@ val _ = translation_extends "basisProg";
 val _ = hide "name";
 
 val evaluate_to_div_limit_def = Define `
-  evaluate_to_div_limit st env exp heap lim_opt =
-    ∃(sts: num->'ffi semanticPrimitives$state) (cks: num->num) io'.
-       (* the heap is a representation of the final io_events *)
-       io2heap io' = heap /\
-       (* clocks increase *)
-       (∀i. cks i < cks (i+1)) /\
-       (* all clocks in the sequence produce timeout and a state in sts *)
-       (∀i. (!n. lim_opt = SOME n ==> cks i < n) ==>
-            evaluate_ck (cks i) st env [exp] =
-              (sts i, Rerr (Rabort Rtimeout_error))) /\
-       (* the limit state st' approximates all states in the sequence *)
-       (∀i. LPREFIX (fromList (sts i).ffi.io_events) io') /\
-       (* if there is a maximal io_event list, then io' is that list *)
-       ∀j. (∀i. (sts i).ffi.io_events ≼ (sts j).ffi.io_events) ==>
-           io' = fromList (sts j).ffi.io_events`;
+  evaluate_to_div_limit st env exp heap lim_opt <=>
+     heap = (UNIV:heap) /\
+     (∀i. (!n. lim_opt = SOME n ==> i < n) ==>
+          ?res. evaluate_ck i st env [exp] =
+                  (res, Rerr (Rabort Rtimeout_error)))`;
 
 val evaluate_to_heap_def = Q.prove(`
   evaluate_to_heap st env exp p heap (r:res) <=>
@@ -36,8 +26,6 @@ val evaluate_to_heap_def = Q.prove(`
         st2heap p st' = heap)
     | Div => evaluate_to_div_limit st env exp heap NONE
     | DivN n => evaluate_to_div_limit st env exp heap (SOME n)`,cheat);
-
-(*
 
 val evaluate_to_heap_Val_11 = store_thm("evaluate_to_heap_Val_11",
   ``!st x0 x1 p heap1 heap2 v1 v2.
@@ -54,11 +42,31 @@ val app_def = prove(
            (POSTv g. H * &app p g (v10::v11) H Q)``,
   cheat);
 
+val POST_DIV_N_simp = prove(
+  ``POST_DIV_N n Qd r h <=> r = DivN n /\ Qd h``,
+  Cases_on `r` \\ fs [POST_DIV_N_def,cond_STAR] \\ fs [cond_def]
+  \\ eq_tac \\ fs []);
+
+val POSTd_simp = prove(
+  ``POSTd Qd r h <=> r = Div /\ Qd h``,
+  Cases_on `r` \\ fs [POSTd_def,cond_STAR] \\ fs [cond_def]
+  \\ eq_tac \\ fs []);
+
+val evaluate_to_heap_UNIV = prove(
+  ``(evaluate_to_heap st env exp p heap (DivN n) <=>
+     evaluate_to_heap st env exp p heap (DivN n) /\ heap = UNIV) /\
+    (evaluate_to_heap st env exp p heap Div <=>
+     evaluate_to_heap st env exp p heap Div /\ heap = UNIV)``,
+  cheat);
+
+val SPLIT3_UNIV_EMPTY = prove(
+  ``SPLIT3 UNIV (∅,h,x) <=> x = UNIV DIFF h``,
+  fs [SPLIT3_def,EXTENSION,IN_DISJOINT] \\ metis_tac []);
+
 val app_POST_DIV_N = store_thm("app_POST_DIV_N",
   ``!xs fv H.
-      (!n. app (p:'ffi ffi_proj) fv xs H (POST_DIV_N n Qd)) =
-      app (p:'ffi ffi_proj) fv xs H (POSTd Qd)``,
-
+      (!n. app (p:'ffi ffi_proj) fv xs H (POST_DIV_N n (&T))) =
+      app (p:'ffi ffi_proj) fv xs H (POSTd (&T))``,
   once_rewrite_tac [EQ_SYM_EQ]
   \\ Induct THEN1 fs [app_def]
   \\ reverse (Cases_on `xs`)
@@ -94,12 +102,13 @@ val app_POST_DIV_N = store_thm("app_POST_DIV_N",
     \\ qexists_tac `DivN n` \\ fs [POST_DIV_N_def,cond_STAR]
     \\ fs [evaluate_to_heap_def,evaluate_to_div_limit_def]
     \\ metis_tac [])
-  \\ first_x_assum drule \\ fs []
-
-  \\ strip_tac \\ asm_exists_tac \\ fs []
-  \\ Cases_on `r` \\ fs [POSTd_def] \\ TRY (fs [cond_def] \\ NO_TAC)
-
-*)
+  \\ first_x_assum drule \\ fs [POST_DIV_N_simp,POSTd_simp]
+  \\ fs [cond_def]
+  \\ once_rewrite_tac [evaluate_to_heap_UNIV] \\ fs [SPLIT3_UNIV_EMPTY]
+  \\ Cases_on `do_opapp [fv; h]` \\ fs []
+  \\ PairCases_on `x` \\ fs []
+  \\ fs [evaluate_to_heap_def,evaluate_to_div_limit_def]
+  \\ rw [] \\ pop_assum match_mp_tac \\ qexists_tac `i+1` \\ fs []);
 
 val app_eq_cf_body = store_thm("app_eq_cf_body",
   ``find_recfun f funs = SOME (param,body) /\
@@ -111,14 +120,7 @@ val app_eq_cf_body = store_thm("app_eq_cf_body",
     app p (Recclosure env funs f) xs H (POST_DIV_N (SUC n) Qd)``,
   rw []
   \\ drule (cf_sound |> SIMP_RULE std_ss [sound_def,htriple_valid_def])
-
-
-  cheat);
-
-
-
-
-
+  \\ cheat);
 
 val app_POST_DIV_N_0 = store_thm("app_POST_DIV_N_0",
   ``xs <> [] /\ find_recfun f funs = SOME (param, body) ==>
@@ -145,8 +147,8 @@ val div_ind = Q.store_thm("div_ind",
                 (MAP (\ (f,_,_). naryRecclosure env
                   (letrec_pull_params funs) f) funs)
               [param] xs env) H (POST_DIV_N n (&T)))) ==>
-     !n. app (p:'ffi ffi_proj) fv xs H (POST_DIV_N n (&T))`,
-  rw [] \\ Induct_on `n`
+     app (p:'ffi ffi_proj) fv xs H (POSTd (&T))`,
+  rw [GSYM app_POST_DIV_N] \\ Induct_on `n`
   THEN1 metis_tac [app_POST_DIV_N_0]
   \\ match_mp_tac (GEN_ALL app_eq_cf_body)
   \\ fs []);
@@ -168,7 +170,7 @@ val _ = (max_print_depth := 15)
 val loop_spec = Q.store_thm ("loop_spec",
   `!xv n.
      app (p:'ffi ffi_proj) ^(fetch_v "loop" s) [xv]
-       emp (POST_DIV_N n &T)`,
+       emp (POSTd &T)`,
   strip_tac
   \\ match_mp_tac div_ind
   \\ EXISTS_TAC env
